IOStream initial work

runtime/test/positive_test.ml
@@ -16,221 +16,59 @@ let make_positive n =
                                  else fun p -> XO (k p)) in
   aux n true (fun p -> p)
 
-let rec serialize_positive_two p =
-  match p with
-  | XI (XI p) ->
-     Serializer_primitives.append (byte_Serializer.serialize '\000')
-                                  (serialize_positive_two p)
-  | XI (XO p) ->
-     Serializer_primitives.append (byte_Serializer.serialize '\001')
-                                  (serialize_positive_two p)
-  | XO (XI p) ->
-     Serializer_primitives.append (byte_Serializer.serialize '\002')
-                                  (serialize_positive_two p)
-  | XO (XO p) ->
-     Serializer_primitives.append (byte_Serializer.serialize '\003')
-                                  (serialize_positive_two p)
-  | XI p ->
-     Serializer_primitives.append (byte_Serializer.serialize '\004')
-                                  (serialize_positive_two p)
-  | XO p ->
-     Serializer_primitives.append (byte_Serializer.serialize '\005')
-                                  (serialize_positive_two p)
-  | XH -> byte_Serializer.serialize '\006'
-
-(* unverified and doesn't correspond to any deserializer *)
-let rec serialize_positive_three p =
-  match p with
-  | XI (XI (XI p)) ->
-     Serializer_primitives.append (byte_Serializer.serialize '\014')
-                                  (serialize_positive_three p)
-  | XI (XI (XO p)) ->
-     Serializer_primitives.append (byte_Serializer.serialize '\013')
-                                  (serialize_positive_three p)
-  | XI (XO (XI p)) ->
-     Serializer_primitives.append (byte_Serializer.serialize '\012')
-                                  (serialize_positive_three p)
-  | XI (XO (XO p)) ->
-     Serializer_primitives.append (byte_Serializer.serialize '\011')
-                                  (serialize_positive_three p)
-  | XO (XI (XI p)) ->
-     Serializer_primitives.append (byte_Serializer.serialize '\010')
-                                  (serialize_positive_three p)
-  | XO (XI (XO p)) ->
-     Serializer_primitives.append (byte_Serializer.serialize '\009')
-                                  (serialize_positive_three p)
-  | XO (XO (XI p)) ->
-     Serializer_primitives.append (byte_Serializer.serialize '\008')
-                                  (serialize_positive_three p)
-  | XO (XO (XO p)) ->
-     Serializer_primitives.append (byte_Serializer.serialize '\007')
-                                  (serialize_positive_three p)
-  | XI (XI p) ->
-     Serializer_primitives.append (byte_Serializer.serialize '\006')
-                                  (serialize_positive_three p)
-  | XI (XO p) ->
-     Serializer_primitives.append (byte_Serializer.serialize '\005')
-                                  (serialize_positive_three p)
-  | XO (XI p) ->
-     Serializer_primitives.append (byte_Serializer.serialize '\004')
-                                  (serialize_positive_three p)
-  | XO (XO p) ->
-     Serializer_primitives.append (byte_Serializer.serialize '\003')
-                                  (serialize_positive_three p)
-  | XI p ->
-     Serializer_primitives.append (byte_Serializer.serialize '\002')
-                                  (serialize_positive_three p)
-  | XO p ->
-     Serializer_primitives.append (byte_Serializer.serialize '\001')
-                                  (serialize_positive_three p)
-  | XH -> byte_Serializer.serialize '\000'
-
 let rec serialize_positive_three p =
   match p with
   | XI (XI (XI p)) -> fun w ->
                       (byte_Serializer.serialize '\014' w;
                        serialize_positive_three p w)
   | XI (XI (XO p)) -> fun w ->
-     (byte_Serializer.serialize '\013' w;
-     serialize_positive_three p w)
+                      (byte_Serializer.serialize '\013' w;
+                       serialize_positive_three p w)
   | XI (XO (XI p)) -> fun w ->
-     (byte_Serializer.serialize '\012' w;
-     serialize_positive_three p w)
+                      (byte_Serializer.serialize '\012' w;
+                       serialize_positive_three p w)
   | XI (XO (XO p)) -> fun w ->
-     (byte_Serializer.serialize '\011' w;
-     serialize_positive_three p w)
+                      (byte_Serializer.serialize '\011' w;
+                       serialize_positive_three p w)
   | XO (XI (XI p)) -> fun w ->
-     (byte_Serializer.serialize '\010' w;
-     serialize_positive_three p w)
+                      (byte_Serializer.serialize '\010' w;
+                       serialize_positive_three p w)
   | XO (XI (XO p)) -> fun w ->
-     (byte_Serializer.serialize '\009' w;
-     serialize_positive_three p w)
+                      (byte_Serializer.serialize '\009' w;
+                       serialize_positive_three p w)
   | XO (XO (XI p)) -> fun w ->
-     (byte_Serializer.serialize '\008' w;
-     serialize_positive_three p w)
+                      (byte_Serializer.serialize '\008' w;
+                       serialize_positive_three p w)
   | XO (XO (XO p)) -> fun w ->
-     (byte_Serializer.serialize '\007' w;
-     serialize_positive_three p w)
+                      (byte_Serializer.serialize '\007' w;
+                       serialize_positive_three p w)
   | XI (XI p) -> fun w ->
-     (byte_Serializer.serialize '\006' w;
-     serialize_positive_three p w)
+                 (byte_Serializer.serialize '\006' w;
+                  serialize_positive_three p w)
   | XI (XO p) -> fun w ->
-     (byte_Serializer.serialize '\005' w;
-     serialize_positive_three p w)
+                 (byte_Serializer.serialize '\005' w;
+                  serialize_positive_three p w)
   | XO (XI p) -> fun w ->
-     (byte_Serializer.serialize '\004' w;
-     serialize_positive_three p w)
+                 (byte_Serializer.serialize '\004' w;
+                  serialize_positive_three p w)
   | XO (XO p) -> fun w ->
-     (byte_Serializer.serialize '\003' w;
-     serialize_positive_three p w)
+                 (byte_Serializer.serialize '\003' w;
+                  serialize_positive_three p w)
   | XI p -> fun w ->
-     (byte_Serializer.serialize '\002' w;
-     serialize_positive_three p w)
+            (byte_Serializer.serialize '\002' w;
+             serialize_positive_three p w)
   | XO p -> fun w ->
-     (byte_Serializer.serialize '\001' w;
-     serialize_positive_three p w)
+            (byte_Serializer.serialize '\001' w;
+             serialize_positive_three p w)
   | XH -> fun w -> byte_Serializer.serialize '\000' w
-
-                                    
-let rec serialize_positive_four p =
-  match p with
-  | XI (XI (XI (XI p))) ->
-     Serializer_primitives.append (byte_Serializer.serialize '\030')
-                                  (serialize_positive_four p)
-  | XI (XI (XI (XO p))) ->
-     Serializer_primitives.append (byte_Serializer.serialize '\029')
-                                  (serialize_positive_four p)
-  | XI (XI (XO (XI p))) ->
-     Serializer_primitives.append (byte_Serializer.serialize '\028')
-                                  (serialize_positive_four p)
-  | XI (XI (XO (XO p))) ->
-     Serializer_primitives.append (byte_Serializer.serialize '\027')
-                                  (serialize_positive_four p)
-  | XI (XO (XI (XI p))) ->
-     Serializer_primitives.append (byte_Serializer.serialize '\026')
-                                  (serialize_positive_four p)
-  | XI (XO (XI (XO p))) ->
-     Serializer_primitives.append (byte_Serializer.serialize '\025')
-                                  (serialize_positive_four p)
-  | XI (XO (XO (XI p))) ->
-     Serializer_primitives.append (byte_Serializer.serialize '\024')
-                                  (serialize_positive_four p)
-  | XI (XO (XO (XO p))) ->
-     Serializer_primitives.append (byte_Serializer.serialize '\023')
-                                  (serialize_positive_four p)
-  | XO (XI (XI (XI p))) ->
-     Serializer_primitives.append (byte_Serializer.serialize '\022')
-                                  (serialize_positive_four p)
-  | XO (XI (XI (XO p))) ->
-     Serializer_primitives.append (byte_Serializer.serialize '\021')
-                                  (serialize_positive_four p)
-  | XO (XI (XO (XI p))) ->
-     Serializer_primitives.append (byte_Serializer.serialize '\020')
-                                  (serialize_positive_four p)
-  | XO (XI (XO (XO p))) ->
-     Serializer_primitives.append (byte_Serializer.serialize '\019')
-                                  (serialize_positive_four p)
-  | XO (XO (XI (XI p))) ->
-     Serializer_primitives.append (byte_Serializer.serialize '\018')
-                                  (serialize_positive_four p)
-  | XO (XO (XI (XO p))) ->
-     Serializer_primitives.append (byte_Serializer.serialize '\017')
-                                  (serialize_positive_four p)
-  | XO (XO (XO (XI p))) ->
-     Serializer_primitives.append (byte_Serializer.serialize '\016')
-                                  (serialize_positive_four p)
-  | XO (XO (XO (XO p))) ->
-     Serializer_primitives.append (byte_Serializer.serialize '\015')
-                                  (serialize_positive_four p)
-  | XI (XI (XI p)) ->
-     Serializer_primitives.append (byte_Serializer.serialize '\014')
-                                  (serialize_positive_four p)
-  | XI (XI (XO p)) ->
-     Serializer_primitives.append (byte_Serializer.serialize '\013')
-                                  (serialize_positive_four p)
-  | XI (XO (XI p)) ->
-     Serializer_primitives.append (byte_Serializer.serialize '\012')
-                                  (serialize_positive_four p)
-  | XI (XO (XO p)) ->
-     Serializer_primitives.append (byte_Serializer.serialize '\011')
-                                  (serialize_positive_four p)
-  | XO (XI (XI p)) ->
-     Serializer_primitives.append (byte_Serializer.serialize '\010')
-                                  (serialize_positive_four p)
-  | XO (XI (XO p)) ->
-     Serializer_primitives.append (byte_Serializer.serialize '\009')
-                                  (serialize_positive_four p)
-  | XO (XO (XI p)) ->
-     Serializer_primitives.append (byte_Serializer.serialize '\008')
-                                  (serialize_positive_four p)
-  | XO (XO (XO p)) ->
-     Serializer_primitives.append (byte_Serializer.serialize '\007')
-                                  (serialize_positive_four p)
-  | XI (XI p) ->
-     Serializer_primitives.append (byte_Serializer.serialize '\006')
-                                  (serialize_positive_four p)
-  | XI (XO p) ->
-     Serializer_primitives.append (byte_Serializer.serialize '\005')
-                                  (serialize_positive_four p)
-  | XO (XI p) ->
-     Serializer_primitives.append (byte_Serializer.serialize '\004')
-                                  (serialize_positive_four p)
-  | XO (XO p) ->
-     Serializer_primitives.append (byte_Serializer.serialize '\003')
-                                  (serialize_positive_four p)
-  | XI p ->
-     Serializer_primitives.append (byte_Serializer.serialize '\002')
-                                  (serialize_positive_four p)
-  | XO p ->
-     Serializer_primitives.append (byte_Serializer.serialize '\001')
-                                  (serialize_positive_four p)
-  | XH -> byte_Serializer.serialize '\000'
-
 
 let test_cheerios p print =
   test_serialize_deserialize p
+(*
                              (fun p -> Serializer_primitives.wire_wrap
                                          (serialize_positive_three p))
+ *)
+                             positive_serialize_top
                              (fun w -> match positive_deserialize_top w with
                                        | Some p -> p
                                        | None -> failwith "Deserialization failed")
@@ -254,8 +92,13 @@ let _ = compare_time_loop make_positive
                           (*
                           positive_serialize_top
                            *)
+
+                          (*
                           (fun p -> Serializer_primitives.wire_wrap
                                       (serialize_positive_three p))
+                           *)
+
+                          positive_serialize_top                          
                           (fun w -> match positive_deserialize_top w with
                                     | Some p -> p
                                     | None -> failwith "Deserialization failed")
