core/Core.v
@@ -5,7 +5,7 @@ Require Import Cheerios.Types.
 
 Set Implicit Arguments.
 
-Module Serializer : SERIALIZER.
+Module Serializer : WRITER.
   Definition t := list byte.
   Definition wire := list byte.
   Axiom wire_eq_dec : forall w w' : wire, {w = w'}+{w <> w'}.
@@ -17,7 +17,7 @@ Module Serializer : SERIALIZER.
 
   Definition unwrap (x : t) : list byte := x.
   Definition wire_wrap (x : t) : wire := x.
-  Definition wire_unwrap (x : wire) : t := x.
+  Definition wire_unwrap (x : wire) : list byte := x.
   
   Lemma empty_unwrap : unwrap empty = [].
   Proof. reflexivity. Qed.
@@ -29,62 +29,14 @@ Module Serializer : SERIALIZER.
     forall x y : t, unwrap (append x y) = unwrap x ++ unwrap y.
   Proof. reflexivity. Qed.
 
-  Lemma wire_wrap_unwrap_inv : forall x, wire_unwrap (wire_wrap x) = x.
+  Lemma wire_wrap_unwrap : forall x, wire_unwrap (wire_wrap x) = unwrap x.
   Proof. reflexivity. Qed.
 End Serializer.
 
 (* This is the monad used to write deserializers. It is a state monad with
     failure, where the state is the serialized bits. *)
 
-Module Type DESERIALIZER.
-  Parameter t : Type -> Type.
-  
-  Parameter getByte : t byte.
-  Parameter unwrap : forall {A}, t A -> list byte -> option (A * list byte).
-
-  Parameter getByte_unwrap : forall l,
-      unwrap getByte l = match l with
-                         | [] => None
-                         | a :: l => Some (a, l)
-                         end.
-
-  Parameter bind : forall {A B}, t A -> (A -> t B) -> t B.
-  Parameter ret : forall {A}, A -> t A.
-  Parameter map : forall {A B}, (A -> B) -> t A -> t B.
-  Parameter error : forall {A}, t A.
-
-  Parameter fold : forall {S A},
-      (byte -> S -> fold_state S A) -> S -> t A.
-
-  Parameter bind_unwrap : forall A B (m : t A)
-                             (f : A -> t B) bytes,
-      unwrap (bind m f) bytes = match unwrap m bytes with
-                                | None => None
-                                | Some (v, bytes) => unwrap (f v) bytes
-                              end.
-  Parameter ret_unwrap : forall A (x: A) bytes, unwrap (ret x) bytes = Some (x, bytes).
-
-  Parameter map_unwrap: forall A B (f: A -> B) (d: t A) bin,
-      unwrap (map f d) bin =
-      match (unwrap d bin) with
-      | None => None
-      | Some (v, bin) => Some (f v, bin)
-      end.
-
-  Parameter fold_unwrap : forall {S A : Type}
-                             (f : byte -> S -> fold_state S A) (s : S) l,
-      unwrap (fold f s) l =
-      match l with
-      | [] => None
-      | b :: l => match f b s with
-                  | Done a => Some (a, l)
-                  | More s => unwrap (fold f s) l
-                  | Error => None
-                  end
-      end.
-End DESERIALIZER.
-
-Module Deserializer : DESERIALIZER.
+Module Deserializer : READER.
   Definition t (A : Type) := list byte -> option (A * list byte).
   Definition unwrap {A} (x : t A) := x.
 
@@ -166,57 +118,4 @@ Module Deserializer : DESERIALIZER.
 End Deserializer.
 Arguments Deserializer.error {_}.
 
-
-
-Notation serialize_deserialize_id_spec s d :=
-  (forall a bytes,
-      Deserializer.unwrap d (Serializer.unwrap (s a) ++ bytes) = Some(a, bytes)).
-
-(* This is the class of serializable types, which is the main entrypoint to
-   Cheerios. Instances are required to show that `deserialize` can correctly
-   recognize a piece of `serialize`d data at the prefix of an arbitrary
-   bitstream. *)
-Class Serializer (A : Type) : Type :=
-  {
-    serialize : A -> Serializer.t;
-    deserialize : Deserializer.t A;
-    serialize_deserialize_id : serialize_deserialize_id_spec serialize deserialize
-  }.
-Hint Rewrite @serialize_deserialize_id : cheerios.
-
-(* In particular, if there is nothing else in the bitsream, then deserialize and
-   serialize are inverses. *)
-Lemma serialize_deserialize_id_nil :
-  forall A (sA : Serializer A) a,
-    Deserializer.unwrap deserialize (Serializer.unwrap (serialize a)) = Some (a, []).
-Proof.
-  intros.
-  pose proof serialize_deserialize_id a [].
-  now rewrite app_nil_r in *.
-Qed.
-
-Section top.
-  Variable A : Type.
-  Variable sA: Serializer A.
-
-  Definition serialize_top (s : A -> Serializer.t) (a : A) : Serializer.wire :=
-    Serializer.wire_wrap (s a).
-
-  Definition deserialize_top
-             (d : Deserializer.t A)
-             (w : Serializer.wire) : option A :=
-    match Deserializer.unwrap d
-                              (Serializer.unwrap (Serializer.wire_unwrap w)) with
-    | None => None
-    | Some (a, _) => Some a
-    end.
-
-  Theorem serialize_deserialize_top_id : forall a,
-      deserialize_top deserialize (serialize_top serialize a) = Some a.
-  Proof.
-    intros.
-    unfold serialize_top, deserialize_top.
-    rewrite Serializer.wire_wrap_unwrap_inv.
-    now rewrite serialize_deserialize_id_nil.
-  Qed.
-End top.
+Module ByteListSerializer := SerializerClass Serializer Deserializer.
