core/Types.v
@@ -31,7 +31,7 @@ Inductive byte :=
 | xea | xeb | xec | xed | xee | xef | xf0 | xf1 | xf2 | xf3 | xf4 | xf5 | xf6
 | xf7 | xf8 | xf9 | xfa | xfb | xfc | xfd | xfe | xff.
 
-Module Type SERIALIZER.
+Module Type WRITER.
   Parameter t : Type.
   Parameter wire : Type.
   Parameter wire_eq_dec : forall w w' : wire, {w = w'}+{w <> w'}.
@@ -43,11 +43,114 @@ Module Type SERIALIZER.
   (* For proof only! Do not call from serializers. *)
   Parameter unwrap : t -> list byte.
   Parameter wire_wrap : t -> wire.
-  Parameter wire_unwrap : wire -> t.
+  Parameter wire_unwrap : wire -> list byte.
 
   Parameter empty_unwrap : unwrap empty = [].
   Parameter append_unwrap :
       forall x y : t, unwrap (append x y) = unwrap x ++ unwrap y.
   Parameter putByte_unwrap : forall (a : byte), unwrap (putByte a) = [a].
-  Parameter wire_wrap_unwrap_inv : forall x, wire_unwrap (wire_wrap x) = x.
-End SERIALIZER.
+  Parameter wire_wrap_unwrap : forall x, wire_unwrap (wire_wrap x) = unwrap x.
+End WRITER.
+
+Module Type READER.
+  Parameter t : Type -> Type.
+  
+  Parameter getByte : t byte.
+  Parameter unwrap : forall {A}, t A -> list byte -> option (A * list byte).
+
+  Parameter getByte_unwrap : forall l,
+      unwrap getByte l = match l with
+                         | [] => None
+                         | a :: l => Some (a, l)
+                         end.
+
+  Parameter bind : forall {A B}, t A -> (A -> t B) -> t B.
+  Parameter ret : forall {A}, A -> t A.
+  Parameter map : forall {A B}, (A -> B) -> t A -> t B.
+  Parameter error : forall {A}, t A.
+
+  Parameter fold : forall {S A},
+      (byte -> S -> fold_state S A) -> S -> t A.
+
+  Parameter bind_unwrap : forall A B (m : t A)
+                             (f : A -> t B) bytes,
+      unwrap (bind m f) bytes = match unwrap m bytes with
+                                | None => None
+                                | Some (v, bytes) => unwrap (f v) bytes
+                              end.
+  Parameter ret_unwrap : forall A (x: A) bytes, unwrap (ret x) bytes = Some (x, bytes).
+
+  Parameter map_unwrap: forall A B (f: A -> B) (d: t A) bin,
+      unwrap (map f d) bin =
+      match (unwrap d bin) with
+      | None => None
+      | Some (v, bin) => Some (f v, bin)
+      end.
+
+  Parameter fold_unwrap : forall {S A : Type}
+                             (f : byte -> S -> fold_state S A) (s : S) l,
+      unwrap (fold f s) l =
+      match l with
+      | [] => None
+      | b :: l => match f b s with
+                  | Done a => Some (a, l)
+                  | More s => unwrap (fold f s) l
+                  | Error => None
+                  end
+      end.
+End READER.
+
+Module SerializerClass (Serializer : WRITER) (Deserializer : READER).
+  Notation serialize_deserialize_id_spec s d :=
+    (forall a bytes,
+        Deserializer.unwrap d (Serializer.unwrap (s a) ++ bytes) = Some(a, bytes)).
+
+  (* This is the class of serializable types, which is the main entrypoint to
+   Cheerios. Instances are required to show that `deserialize` can correctly
+   recognize a piece of `serialize`d data at the prefix of an arbitrary
+   bitstream. *)
+  Class Serializer (A : Type) : Type :=
+    {
+      serialize : A -> Serializer.t;
+      deserialize : Deserializer.t A;
+      serialize_deserialize_id : serialize_deserialize_id_spec serialize deserialize
+    }.
+  Hint Rewrite @serialize_deserialize_id : cheerios.
+
+  (* In particular, if there is nothing else in the bitsream, then deserialize and
+   serialize are inverses. *)
+  Lemma serialize_deserialize_id_nil :
+    forall A (sA : Serializer A) a,
+      Deserializer.unwrap deserialize (Serializer.unwrap (serialize a)) = Some (a, []).
+  Proof.
+    intros.
+    pose proof serialize_deserialize_id a [].
+    now rewrite app_nil_r in *.
+  Qed.
+
+  Section top.
+    Variable A : Type.
+    Variable sA: Serializer A.
+
+    Definition serialize_top (s : A -> Serializer.t) (a : A) : Serializer.wire :=
+      Serializer.wire_wrap (s a).
+
+    Definition deserialize_top
+               (d : Deserializer.t A)
+               (w : Serializer.wire) : option A :=
+      match Deserializer.unwrap d
+                                (Serializer.wire_unwrap w) with
+      | None => None
+      | Some (a, _) => Some a
+      end.
+
+    Theorem serialize_deserialize_top_id : forall a,
+        deserialize_top deserialize (serialize_top serialize a) = Some a.
+    Proof.
+      intros.
+      unfold serialize_top, deserialize_top.
+      rewrite Serializer.wire_wrap_unwrap.
+      now rewrite serialize_deserialize_id_nil.
+    Qed.
+  End top.
+End SerializerClass.
