core/DeserializerMonad.v
@@ -1,58 +1,61 @@
 Require Import Cheerios.Core.
+Require Import Cheerios.Types.
 Require Import List.
 Import ListNotations.
 
-Definition sequence {A B} (df : Deserializer.t (A -> B))
-           (da : Deserializer.t A) : Deserializer.t B :=
-  Deserializer.bind df
-                    (fun f =>
-                          (Deserializer.bind da
-                                             (fun a => Deserializer.ret (f a)))).
+Module DeserializerMonad (Reader : READER).
+  Definition sequence {A B} (df : Reader.t (A -> B))
+             (da : Reader.t A) : Reader.t B :=
+    Reader.bind df
+                (fun f =>
+                   (Reader.bind da
+                                (fun a => Reader.ret (f a)))).
 
-Lemma sequence_rewrite : forall {A B : Type}
-                                (df : Deserializer.t (A -> B))
-                                (da : Deserializer.t A),
-  sequence df da =
-  Deserializer.bind df
-                    (fun f =>
-                       (Deserializer.bind da
-                                          (fun a => Deserializer.ret (f a)))).
-Proof.
-  reflexivity.
-Qed.
-Hint Rewrite @sequence_rewrite : cheerios.
+  Lemma sequence_rewrite : forall {A B : Type}
+                                  (df : Reader.t (A -> B))
+                                  (da : Reader.t A),
+      sequence df da =
+      Reader.bind df
+                  (fun f =>
+                     (Reader.bind da
+                                  (fun a => Reader.ret (f a)))).
+  Proof.
+    reflexivity.
+  Qed.
+  Hint Rewrite @sequence_rewrite : cheerios.
 
-Module DeserializerNotations.
-  Notation "m >>= f" := (@Deserializer.bind _ _ m f) (at level 42, left associativity).
+  Module DeserializerNotations.
+    Notation "m >>= f" := (@Reader.bind _ _ m f) (at level 42, left associativity).
 
-  Notation "x <- c1 ;; c2" := (c1 >>= (fun x => c2))
-                                (at level 100, c1 at next level, right associativity).
-  Notation "e1 ;; e2" := (_ <- e1 ;; e2)
-                            (at level 100, right associativity).
+    Notation "x <- c1 ;; c2" := (c1 >>= (fun x => c2))
+                                  (at level 100, c1 at next level, right associativity).
+    Notation "e1 ;; e2" := (_ <- e1 ;; e2)
+                             (at level 100, right associativity).
 
-  Notation "f <$> x" := (@Deserializer.map _ _ f x) (at level 42, left associativity).
+    Notation "f <$> x" := (@Reader.map _ _ f x) (at level 42, left associativity).
 
-  Notation "f <*> x" := (@sequence _ _ f x) (at level 42, left associativity).
-End DeserializerNotations.
+    Notation "f <*> x" := (@sequence _ _ f x) (at level 42, left associativity).
+  End DeserializerNotations.
 
-Check sequence.
-Import DeserializerNotations.
+  Check sequence.
+  Import DeserializerNotations.
 
-Section lift.
-  Context {A B C D : Type}.
-  Context {sA : Serializer A}.
-  Context {sB : Serializer B}.
-  Context {sC : Serializer C}.
-  Context {sD : Serializer D}.
-  Definition liftD1 {X} (f : D -> X) :=
-    f <$> deserialize.
+  Section lift.
+    Import ByteListSerializer.
+    Context {A B C D : Type}.
+    Context {sA : Serializer A}.
+    Context {sB : Serializer B}.
+    Context {sC : Serializer C}.
+    Context {sD : Serializer D}.
+    Definition liftD1 {X} (f : D -> X) :=
+      f <$> deserialize.
 
-  Definition liftD2 {X} (f : C -> D -> X) : Deserializer.t X :=
-    (f <$> deserialize) >>= liftD1.
+    Definition liftD2 {X} (f : C -> D -> X) : Reader.t X :=
+      (f <$> deserialize) >>= liftD1.
 
-  Definition liftD3 {X} (f : B -> C -> D -> X) : Deserializer.t X :=
-    (f <$> deserialize) >>= liftD2.
+    Definition liftD3 {X} (f : B -> C -> D -> X) : Reader.t X :=
+      (f <$> deserialize) >>= liftD2.
 
-  Definition liftD4 {X} (f : A -> B -> C -> D -> X) : Deserializer.t X :=
-    (f <$> deserialize) >>= liftD3.
-End lift.
+    Definition liftD4 {X} (f : A -> B -> C -> D -> X) : Reader.t X :=
+      (f <$> deserialize) >>= liftD3.
+  End lift.
