core/IOStream.v
@@ -1,0 +1,60 @@
+Require Import Cheerios.Core.
+Require Import Cheerios.Types.
+
+Require Import List.
+Import ListNotations.
+
+Module IOStream : WRITER.
+  Inductive iostream :=
+  | Done : iostream
+  | WriteByte : byte -> (unit -> iostream) -> iostream
+  | Seq : iostream -> iostream -> iostream.
+
+  Definition t := iostream.
+
+  Fixpoint iostreamDenote (i : iostream) : list byte :=
+    match i with
+    | Done => []
+    | WriteByte b thunk => b :: iostreamDenote (thunk tt)
+    | Seq i1 i2 => iostreamDenote i1 ++ iostreamDenote i2
+    end.
+
+  Definition unwrap := iostreamDenote.
+
+  (* serializers *)
+  Definition empty : iostream := Done.
+
+  Definition putByte : byte -> iostream :=
+    fun b => WriteByte b (fun _ => Done).
+
+  Fixpoint putList (l : list byte) :  iostream :=
+    match l with
+    | [] => Done
+    | b :: l => WriteByte b (fun _ => putList l)
+    end.
+
+  Definition append : iostream -> iostream -> iostream := Seq.
+
+  Lemma empty_unwrap : unwrap empty = [].
+  Proof. reflexivity. Qed.
+    
+  Lemma append_unwrap :
+    forall x y : t, unwrap (append x y) = unwrap x ++ unwrap y.
+  Proof. reflexivity. Qed.
+  
+  Lemma putByte_unwrap : forall (a : byte), unwrap (putByte a) = [a].
+  Proof. reflexivity. Qed.
+
+  Definition wire := list byte.
+
+  Axiom wire_eq_dec : forall w w' : wire, {w = w'} + {w <> w'}.
+
+  Definition wire_wrap := unwrap.
+
+  Definition wire_unwrap (x : wire) := x.
+
+  Lemma wire_wrap_unwrap : forall x, wire_unwrap (wire_wrap x) = unwrap x.
+  Proof. reflexivity. Qed.
+End IOStream.
+
+Module IOStreamSerializer := SerializerClass IOStream Deserializer.
