core/Tactics.v
@@ -2,11 +2,18 @@ Require Import List.
 
 Require Import Cheerios.Core.
 Require Import Cheerios.DeserializerMonad.
+Require Import Cheerios.IOStream.
+Require Import Cheerios.Types.
 
 Ltac cheerios_crush := intros; autorewrite with cheerios; auto.
 
-Hint Rewrite app_ass 
-     Serializer.empty_unwrap Serializer.putByte_unwrap
-     Serializer.append_unwrap Deserializer.getByte_unwrap
-     Deserializer.bind_unwrap Deserializer.ret_unwrap
-     Deserializer.map_unwrap @Deserializer.fold_unwrap : cheerios.
+Module WriterRewrite (Writer : WRITER).
+  Hint Rewrite app_ass 
+       Writer.empty_unwrap Writer.putByte_unwrap
+       Writer.append_unwrap : cheerios.
+End WriterRewrite.
+
+Module ReaderRewrite (Reader : READER).
+  Hint Rewrite Reader.getByte_unwrap Reader.bind_unwrap Reader.ret_unwrap
+       Reader.map_unwrap @Reader.fold_unwrap : cheerios.
+End ReaderRewrite.
