runtime/coq/ExtractPositiveSerializer.v
@@ -4,11 +4,17 @@ Require Import ZArith.
 Require Import ExtrOcamlBasic.
 Require Import ExtrOcamlString.
 
+Import ByteListSerializer.
+
 Definition positive_serialize_top : positive -> Serializer.wire :=
-  serialize_top (serialize : positive -> Serializer.t).
+  serialize_top _ serialize.
+
+Definition positive_serialize_top_tr :=
+  serialize_top _ (fun p => positive_serialize_rec p Serializer.empty).
 
 Definition positive_deserialize_top : Serializer.wire -> option positive :=
-  deserialize_top (deserialize : Deserializer.t positive).
+  deserialize_top _ (deserialize : Deserializer.t positive).
 
 Extraction "runtime/ocaml/positive_serializer.ml"
-           positive_serialize_top positive_deserialize_top.
+           positive_serialize_top positive_deserialize_top
+           positive_serialize_top_tr.
